Z.lean
@@ -1,6 +1,7 @@
 import Z.Interpreter
 import Z.DefaultServices
 import Z.Layer
+import Z.Do
 
 
 namespace Fiber
